Reorganize

Imp.lean
@@ -1,348 +1,29 @@
 import Lean.PrettyPrinter.Delaborator
 import LeanSAT.Reflect.Tactics.BVDecide
 
-abbrev Value := BitVec 32
+import Imp.Expr
+import Imp.Expr.Eval
+import Imp.Expr.Optimize
+import Imp.Expr.Delab
 
-def Env := String → Value
+import Imp.Stmt
+import Imp.Stmt.Delab
 
-def Env.set (x : String) (v : Value) (ρ : Env) : Env :=
-  fun y => if x == y then v else ρ y
-
-def Env.get (x : String) (ρ : Env) : Value :=
-  ρ x
-
-def Env.init (i : Value) : Env := fun _ => i
-
-inductive UnOp where
-  | neg
-  | not
-deriving Repr, DecidableEq
-
-inductive BinOp where
-  | plus | minus | times | div
-  | lsh | rsh
-  | band | bor
-  | and | or
-  | lt | le | eq
-deriving Repr, DecidableEq
-
-inductive Expr where
-  | const (i : Value)
-  | var (name : String)
-  | un (op : UnOp) (e : Expr)
-  | bin (op : BinOp) (e1 e2 : Expr)
-deriving Repr, DecidableEq
-
-declare_syntax_cat varname
-syntax ident : varname
-syntax "~" term : varname
-
-syntax "var " "{" varname "}" : term
-
-open Lean in
-macro_rules
-  | `(var { $x:ident }) => `(term|$(quote x.getId.toString))
-  | `(var { ~$stx }) => pure stx
-
-namespace Expr.Syntax
-declare_syntax_cat exp
-syntax varname : exp
-/-- Numeric constant -/
-syntax num : exp
-/-- Arithmetic complement -/
-syntax:75 "-" exp:75 : exp
-/-- Addition -/
-syntax:65 exp:65 " + " exp:66 : exp
-/-- Multiplication -/
-syntax:70 exp:70 " * " exp:71 : exp
-/-- Subtraction -/
-syntax:65 exp:65 " - " exp:66 : exp
-/-- Division -/
-syntax:65 exp:65 " / " exp:66 : exp
-
--- todo precs
-syntax:55 exp:55 " <<< " exp:56 :exp
-syntax:55 exp:55 " >>> " exp:56 :exp
-syntax:55 exp:55 " &&& " exp:56 :exp
-syntax:55 exp:55 " ||| " exp:56 :exp
-
---todo precs for these
-/-- Boolean conjunction -/
-syntax:65 exp:65 " && " exp:66 : exp
-/-- Boolean disjunction -/
-syntax:65 exp:65 " || " exp:66 : exp
-
-/-- Boolean negation -/
-syntax:75 "!" exp:75 : exp
-/-- Less than -/
-syntax:50 exp:50 " < " exp:50 : exp
-/-- Less than or equal to -/
-syntax:50 exp:50 " ≤ " exp:50 : exp
-/-- Equal -/
-syntax:50 exp:50 " = " exp:50 : exp
-/-- Equal -/
-syntax:50 exp:50 " == " exp:50 : exp
-/-- Greater than or equal to -/
-syntax:50 exp:50 " ≥ " exp:50 : exp
-/-- Greater than -/
-syntax:50 exp:50 " > " exp:50 : exp
-
-/-- Parens -/
-syntax "(" exp ")" : exp
-
-syntax "~" term : exp
-
-syntax "lean " "{" term "}" : exp
-
-syntax "expr" "{" exp "}" : term
-
-open Lean in
-macro_rules
-  | `(expr{$x:ident}) => `(Expr.var $(quote x.getId.toString))
-  | `(expr{$n:num}) => `(Expr.const $(quote n.getNat))
-
-  | `(expr{-$e}) => `(Expr.un .neg expr{$e})
-  | `(expr{!$e}) => `(Expr.un .not expr{$e})
-
-  | `(expr{$e1 + $e2}) => `(Expr.bin .plus expr{$e1} expr{$e2})
-  | `(expr{$e1 * $e2}) => `(Expr.bin .times expr{$e1} expr{$e2})
-  | `(expr{$e1 - $e2}) => `(Expr.bin .minus expr{$e1} expr{$e2})
-  | `(expr{$e1 / $e2}) => `(Expr.bin .div expr{$e1} expr{$e2})
-
-  | `(expr{$e1 >>> $e2}) => `(Expr.bin .rsh expr{$e1} expr{$e2})
-  | `(expr{$e1 <<< $e2}) => `(Expr.bin .lsh expr{$e1} expr{$e2})
-  | `(expr{$e1 ||| $e2}) => `(Expr.bin .bor expr{$e1} expr{$e2})
-  | `(expr{$e1 &&& $e2}) => `(Expr.bin .band expr{$e1} expr{$e2})
-
-
-  | `(expr{$e1 && $e2}) => `(Expr.bin .and expr{$e1} expr{$e2})
-  | `(expr{$e1 || $e2}) => `(Expr.bin .or expr{$e1} expr{$e2})
-
-  | `(expr{$e1 < $e2}) => `(Expr.bin .lt expr{$e1} expr{$e2})
-  | `(expr{$e1 ≤ $e2}) => `(Expr.bin .le expr{$e1} expr{$e2})
-  | `(expr{$e1 == $e2}) => `(Expr.bin .eq expr{$e1} expr{$e2})
-  | `(expr{$e1 ≥ $e2}) => `(Expr.bin .le expr{$e2} expr{$e1})
-  | `(expr{$e1 > $e2}) => `(Expr.bin .lt expr{$e2} expr{$e1})
-  | `(expr{($e)}) => `(expr{$e})
-  | `(expr{~$stx}) => pure stx
-
-end Expr.Syntax
-
-def Expr.freeVars : Expr → List String
-  | .const _ => []
-  | .var x => [x]
-  | .un _ e => e.freeVars
-  | .bin _ e1 e2 => e1.freeVars ++ e2.freeVars
-
-def UnOp.apply : UnOp → Value → Option Value
-  | .neg, x => some (- x)
-  | .not, x => some (if x == 0 then 1 else 0)
-
-def BinOp.apply : BinOp → Value → Value → Option Value
-  | .plus, x, y => some (x + y)
-  | .minus, x, y => some (x - y)
-  | .times, x, y => some (x * y)
-  | .lsh, x, y => some (x <<< y)
-  | .rsh, x, y => some (x >>> y)
-  | .band, x, y => some (x &&& y)
-  | .bor, x, y => some (x ||| y)
-  | .div, x, y => if y == 0 then none else some (x / y)
-  | .and, x, y => some (if x == 0 then 0 else y)
-  | .or, x, y => some (if x == 0 then y else x)
-  | .eq, x, y => some (if x == y then 1 else 0)
-  | .le, x, y => some (if x ≤ y then 1 else 0)
-  | .lt, x, y => some (if x < y then 1 else 0)
-
-def Expr.eval (ρ : Env) : Expr → Option Value
-  | .const i => some i
-  | .var x => ρ x
-  | .un op e => do
-    let v ← e.eval ρ
-    op.apply v
-  | .bin op e1 e2 => do
-    let v1 ← e1.eval ρ
-    let v2 ← e2.eval ρ
-    op.apply v1 v2
-
-def Expr.optimize : Expr → Expr
-  | .const i => .const i
-  | .var x => .var x
-  | .un op e =>
-    match optimize e with
-    | .const i =>
-      if let some v := op.apply i then .const v
-      else .un op (.const i)
-    | e' => .un op e'
-  | .bin op e1 e2 =>
-    match optimize e1, optimize e2 with
-    | .const i, .const i' =>
-      if let some v := op.apply i i' then .const v
-      else .bin op (.const i) (.const i')
-    | e1', e2' => .bin op e1' e2'
-
-theorem Expr.optimize_ok (e : Expr) : e.eval ρ = e.optimize.eval ρ := by
-  induction e <;> simp [optimize]
-  next op e ih =>
-    split <;> simp [eval, *]
-    cases op <;> simp [UnOp.apply, eval]
-  next op e1 e2 ih1 ih2 =>
-    split <;> simp [eval, *]
-    cases op <;> simp [BinOp.apply, eval]
-    split
-    . simp [eval, BinOp.apply]; split <;> trivial
-    . simp [eval]
-
-inductive Stmt where
-  | skip
-  | seq (stmt1 stmt2 : Stmt)
-  | assign (name : String) (val : Expr)
-  | if (cond : Expr) (ifTrue ifFalse : Stmt)
-  | while (cond : Expr) (body : Stmt)
-deriving Repr, DecidableEq
-
-namespace Stmt.Syntax
-declare_syntax_cat stmt
-scoped syntax "skip" : stmt
-scoped syntax stmt ";" ppDedent(ppLine stmt) : stmt
-scoped syntax varname " := " exp : stmt
-scoped syntax "if " "(" exp ")" "{" ppIndent(ppLine stmt) ppLine "}" " else " "{" ppIndent(ppLine stmt) ppLine "}" : stmt
-scoped syntax ppAllowUngrouped "while " "(" exp ")" ppHardSpace "{" ppIndent(ppLine stmt) ppLine "}" : stmt
-scoped syntax ppAllowUngrouped ppDedentIfGrouped("lean" ppHardSpace ppGroup("{ " ppLine term ppDedent(ppLine) " }")) : stmt
-scoped syntax "~" term : stmt
-
-syntax "program" ppHardSpace "{" ppLine stmt ppDedent(ppLine) "}" : term
-
-
-open Lean in
-macro_rules
-  | `(program { skip }) => `(Stmt.skip)
-  | `(program { $s1; $s2 }) => `(Stmt.seq program {$s1} program {$s2})
-  | `(program { $x:varname := $e}) =>
-      `(Stmt.assign var {$x} expr {$e})
-  | `(program { if ($c) {$s1} else {$s2} }) => `(Stmt.if expr{$c} program{$s1} program{$s2})
-  | `(program { while ($c) {$s} }) => `(Stmt.while expr{$c} program{$s})
-  | `(program { ~$stx }) => pure stx
+namespace Imp
 
 open Lean PrettyPrinter Delaborator SubExpr Parenthesizer
 
--- Shamelessly stolen from Lean's term parenthesizer
-@[category_parenthesizer exp]
-def exp.parenthesizer : CategoryParenthesizer | prec => do
-  maybeParenthesize `exp true wrapParens prec $
-    parenthesizeCategoryCore `exp prec
-where
-  wrapParens (stx : Syntax) : Syntax := Unhygienic.run do
-    let pstx ← `(($(⟨stx⟩)))
-    return pstx.raw.setInfo (SourceInfo.fromRef stx)
+open Stmt
 
-@[delab app.Stmt.skip, delab app.Stmt.seq, delab app.Stmt.while, delab app.Stmt.assign, delab App.Stmt.if]
-partial def delabStmt : Delab := do
-  -- This delaborator only understands a certain arity - bail if it's incorrect
-  guard <| match_expr ← getExpr with
-    | Stmt.skip => true
-    | Stmt.seq _ _ => true
-    | Stmt.while _ _ => true
-    | Stmt.assign _ _ => true
-    | Stmt.if _ _ _ => true
-    | _ => false
-  let stx' ← delabStmt
-  if stx'.raw.isAntiquot then
-    let stx := stx'.raw.getAntiquotTerm
-    pure ⟨stx⟩
-  else
-    `(term|program{$stx'})
-where
-  annAsTerm {any} (stx : TSyntax any) : DelabM (TSyntax any) :=
-    (⟨·⟩) <$> annotateTermInfo ⟨stx.raw⟩
-  delabName : DelabM (TSyntax `varname) := do
-    let e ← getExpr
-    match e with
-    | .lit (.strVal s) =>
-      let x := mkIdent <| .mkSimple s
-      pure <| ⟨x.raw⟩
-    | _ => `(varname|~$(← delab)) >>= annAsTerm
-  delabExpr : DelabM (TSyntax `exp) := do
-    let e ← getExpr
-    let stx ←
-      match_expr e with
-      | Expr.const x =>
-        match_expr x with
-        | Int.ofNat n =>
-          if let some n' := n.nat? then
-            pure <| ⟨Syntax.mkNumLit (toString n') |>.raw⟩
-          else if let .lit (.natVal n') := n then
-            pure <| ⟨Syntax.mkNumLit (toString n') |>.raw⟩
-          else withAppArg `(exp| ~$(← delab))
-        | BitVec.ofFin _w f => `(exp|99)
-        | _ => withAppArg `(exp| ~$(← delab))
-      | Expr.var _ => do
-        let x ← withAppArg delabName
-        `(exp|$x:varname)
-      | Expr.bin op _ _ =>
-        let s1 ← withAppFn <| withAppArg delabExpr
-        let s2 ← withAppArg delabExpr
-        match_expr op with
-        | BinOp.plus => `(exp| $s1 + $s2)
-        | BinOp.minus => `(exp| $s1 - $s2)
-        | BinOp.times => `(exp| $s1 * $s2)
-        | BinOp.div => `(exp| $s1 / $s2)
-        | BinOp.and => `(exp| $s1 && $s2)
-        | BinOp.or => `(exp| $s1 || $s2)
-        | BinOp.lt => `(exp| $s1 < $s2)
-        | BinOp.lt => `(exp| $s1 ≤ $s2)
-        | BinOp.lt => `(exp| $s1 == $s2)
-        | _ => `(exp| ~$(← delab))
-      | Expr.un op _ =>
-        let s ← withAppArg delabExpr
-        match_expr op with
-        | UnOp.neg => `(exp|-$s)
-        | UnOp.not => `(exp|!$s)
-        | _ => `(exp| ~$(← delab))
-      | _ => `(exp| ~$(← delab))
-    annAsTerm stx
-  delabStmt : DelabM (TSyntax `stmt) := do
-    let e ← getExpr
-    let stx ←
-      match_expr e with
-      | Stmt.skip => `(stmt| skip)
-      | Stmt.seq _ _ =>
-        let s1 ← withAppFn <| withAppArg delabStmt
-        let s2 ← withAppArg delabStmt
-        `(stmt| $s1 ; $s2)
-      | Stmt.assign _ _ =>
-        let x ← withAppFn <| withAppArg delabName
-        let e ← withAppArg delabExpr
-        `(stmt| $x:varname := $e)
-      | Stmt.while _ _ =>
-        let c ← withAppFn <| withAppArg delabExpr
-        let body ← withAppArg delabStmt
-        `(stmt| while ($c) { $body })
-      | Stmt.if _ _ _ =>
-        let c ← withAppFn <| withAppFn <| withAppArg delabExpr
-        let t ← withAppFn <| withAppArg delabStmt
-        let f ← withAppArg delabStmt
-        `(stmt| if ($c) { $t } else { $f })
-      | _ =>
-        `(stmt| ~$(← delab))
-    annAsTerm stx
+open BitVec
 
-
-
-end Stmt.Syntax
-
-set_option pp.rawOnError true
-
-open Stmt.Syntax in
-#reduce fun s => program {skip; ~s}
-
-open Stmt.Syntax in
 def Stmt.optimize : Stmt → Stmt
-  | program {skip} => program {skip}
-  | program {~s1; ~s2} =>
+  | program {skip;} => program {skip;}
+  | program {~s1 ~s2} =>
     match s1.optimize, s2.optimize with
-    | program {skip}, s2' => s2'
-    | s1', program {skip} => s1'
-    | s1', s2' => program {~s1'; ~s2'}
+    | program {skip;}, s2' => s2'
+    | s1', program {skip;} => s1'
+    | s1', s2' => program {~s1' ~s2'}
   | program {if (~c) {~s1} else {~s2}} =>
     let c' := c.optimize
     match c' with
@@ -357,120 +38,85 @@ def Stmt.optimize : Stmt → Stmt
   | program {while (~c) {~s}} =>
     let c' := c.optimize
     match c' with
-    | .const 0 => program {skip}
+    | .const 0 => program {skip;}
     | _ => program {while (~c') {~s.optimize}}
-  | program {~x := ~e} =>
-    program {~x := ~e.optimize}
+  | program {~x := ~e;} =>
+    program {~x := ~e.optimize;}
 
+def Truthy (v : Option Value) : Prop :=
+  match v with
+  | some v => v ≠ 0
+  | none => False
 
-
-
-inductive IsSkip : (s : Stmt) → Prop where
-  | isSkip : IsSkip .skip
-
-instance : DecidablePred IsSkip := by
-  intro s
-  cases s
-  case skip => apply isTrue; constructor
-  all_goals
-    apply isFalse; intro h; cases h
-
-def AsBool (ρ : Env) (e : Expr) (b : Bool) : Prop :=
-  ∃ v, e.eval ρ = some v ∧ (b = true ↔ v ≠ 0)
-
-open BitVec
-
-instance : Decidable (AsBool ρ e b) :=
-  match h : e.eval ρ with
-  | none => .isFalse <| by intro ⟨v, ⟨p1, p2⟩⟩; rw [h] at p1; cases p1
+instance : Decidable (Truthy v) :=
+  match v with
   | some v =>
-    if h' : v ≠ 0#32 then
-      match b with
-      | true => .isTrue ⟨v, ⟨h, by simp [*]⟩⟩
-      | false => .isFalse <| by
-        intro ⟨v', ⟨x, y⟩⟩
-        rw [h] at x; cases x
-        have := y.mpr h'
-        cases this
-    else
-      match b with
-      | true => .isFalse <| by
-        intro ⟨v', ⟨x, y⟩⟩
-        rw [h] at *; cases h; cases x
-        have := y.mp rfl
-        contradiction
-      | false => .isTrue ⟨v, ⟨h, by simp [*]⟩⟩
+    if h : v ≠ 0 then .isTrue h else .isFalse h
+  | none => .isFalse id
 
-open Stmt.Syntax in
+@[simp]
+theorem Truthy.some_nonzero : Truthy (some v) = (v ≠ 0) := by
+  simp [Truthy]
+
+@[simp]
+theorem Truthy.eval_const : Truthy (Expr.eval ρ (.const v)) = (v ≠ 0) := by
+  simp [Truthy, Expr.eval]
+
+def Falsy (v : Option Value) : Prop := v = some 0
+
+@[simp]
+theorem Falsy.eval_const : Falsy (Expr.eval ρ (.const v)) = (v = 0) := by
+  simp [Falsy, Expr.eval]
+
+@[simp]
+theorem Falsy.some_zero : Falsy (some v) = (v = 0) := by
+  simp [Falsy]
+
+@[simp]
+theorem Falsy.some_const : Falsy (some (BitVec.ofNat _ n)) → (n % 2 ^ 32 = 0) := by
+  simp [Falsy, BitVec.ofNat]
+  unfold Fin.ofNat'
+  rw [← Fin.val_inj]
+  simp
+
+
+
+
+instance : Decidable (Falsy v) := inferInstanceAs (Decidable (v = some 0))
+
+
 inductive BigStep : Env → Stmt → Env → Prop where
   | skip :
-    BigStep ρ (program {skip}) ρ
+    BigStep ρ (program {skip;}) ρ
   | seq :
     BigStep ρ s1 ρ' → BigStep ρ' s2 ρ'' →
-    BigStep ρ (program{ ~s1; ~s2}) ρ''
+    BigStep ρ (program{ ~s1 ~s2}) ρ''
   | assign :
     e.eval ρ = some v →
-    BigStep ρ (program {~x := ~e}) (ρ.set x v)
+    BigStep ρ (program {~x := ~e;}) (ρ.set x v)
   | ifTrue :
-    AsBool ρ c true → BigStep ρ s1 ρ' →
+    Truthy (c.eval ρ) → BigStep ρ s1 ρ' →
     BigStep ρ (program {if (~c) {~s1} else {~s2}}) ρ'
   | ifFalse :
-    AsBool ρ c false → BigStep ρ s2 ρ' →
+    Falsy (c.eval ρ) → BigStep ρ s2 ρ' →
     BigStep ρ (program {if (~c) {~s1} else {~s2}}) ρ'
   | whileTrue :
-    AsBool ρ c true →
+    Truthy (c.eval ρ) →
     BigStep ρ body ρ' →
     BigStep ρ' (program {while (~c) {~body}}) ρ'' →
     BigStep ρ (program {while (~c) {~body}}) ρ''
   | whileFalse :
-    AsBool ρ c false →
+    Falsy (c.eval ρ) →
     BigStep ρ (program {while (~c) {~body}}) ρ
 
-theorem AsBool.optimize_ok : AsBool ρ e b ↔ AsBool ρ e.optimize b := by
-  constructor
-  . intro ⟨v, hasVal, truthy⟩
-    exists v
-    constructor
-    . rw [← Expr.optimize_ok]
-      assumption
-    . assumption
-  . intro ⟨v, hasVal, truthy⟩
-    exists v
-    constructor
-    . rw [Expr.optimize_ok]
-      assumption
-    . assumption
+attribute [simp] BigStep.skip
 
 
-open Stmt.Syntax in
-def loop := program {while (1) {skip}}
 
-open Stmt.Syntax in
+def loop := program {while (1) {skip;}}
+
 def loopOf (s) := program {while (1) {~s}}
 
-
-
-@[simp]
-theorem AsBool.const_false : AsBool ρ (.const i) false → i = 0 := by
-  intro ⟨v, val, b⟩
-  simp [Expr.eval] at val
-  simp at b
-  simp [*]
-
-@[simp]
-theorem AsBool.not_const_1_false : ¬AsBool ρ (.const 1) false := by
-  intro h
-  have := h.const_false
-  cases this
-
-@[simp]
-theorem AsBool.not_const_0_true : ¬AsBool ρ (.const 0) true := by
-  intro ⟨v, val, b⟩
-  simp [Expr.eval] at *
-  rw [val] at b
-  contradiction
-
-open Stmt.Syntax in
 theorem Stmt.infinite_loop : ¬ BigStep ρ loop ρ' := by
   generalize h' : loop = l
   intro h
@@ -480,10 +126,8 @@ theorem Stmt.infinite_loop : ¬ BigStep ρ loop ρ' := by
   | whileFalse cFalse =>
     unfold loop at h'
     cases h'
-    apply cFalse.not_const_1_false
+    cases cFalse
 
-open Stmt.Syntax in
-open BitVec in
 theorem Stmt.infinite_loopOf : ¬ BigStep ρ (loopOf s) ρ' := by
   generalize h' : loopOf s = l
   intro h
@@ -493,23 +137,20 @@ theorem Stmt.infinite_loopOf : ¬ BigStep ρ (loopOf s) ρ' := by
   | whileFalse cFalse =>
     unfold loopOf at h'
     cases h'
-    cases cFalse.not_const_1_false
-
+    cases cFalse
 
 theorem Stmt.optimize_ok : BigStep ρ s ρ' → BigStep ρ s.optimize ρ' := by
   intro h
   induction h with simp only [optimize]
-  | skip => constructor
+  | «skip» => constructor
   | seq s1 s2 ih1 ih2 =>
     split
     next eq2 =>
       rw [eq2] at ih1
-      cases ih1
-      apply ih2
+      cases ih1; apply ih2
     next eq1 eq2 =>
       rw [eq1] at ih2
-      cases ih2
-      apply ih1
+      cases ih2; apply ih1
     next =>
       apply BigStep.seq ih1 ih2
   | assign m =>
@@ -519,16 +160,16 @@ theorem Stmt.optimize_ok : BigStep ρ s ρ' → BigStep ρ s.optimize ρ' := by
   | ifTrue isTrue l ih =>
     split
     next isFalse =>
-      rw [AsBool.optimize_ok] at isTrue
+      rw [Expr.optimize_ok] at isTrue
       rw [isFalse] at isTrue
-      cases isTrue.not_const_0_true
-    next notFalse isConst =>
+      simp [Truthy, Expr.eval] at isTrue
+    next notFalse _isConst =>
       apply ih
     next =>
       split
       . assumption
       . apply BigStep.ifTrue
-        . rw [← AsBool.optimize_ok]
+        . rw [← Expr.optimize_ok]
           assumption
         . assumption
   | ifFalse isFalse l ih =>
@@ -536,85 +177,78 @@ theorem Stmt.optimize_ok : BigStep ρ s ρ' → BigStep ρ s.optimize ρ' := by
     next =>
       apply ih
     next nonZero isConst =>
-      rw [AsBool.optimize_ok, isConst] at isFalse
-      have := isFalse.const_false
-      cases nonZero this
+      rw [Expr.optimize_ok, isConst] at isFalse
+      simp at isFalse
+      contradiction
     next =>
       split
       . simp [*]
       . apply BigStep.ifFalse
-        . rw [← AsBool.optimize_ok]
+        . rw [← Expr.optimize_ok]
           assumption
         . assumption
   | whileFalse =>
-    split
-    next =>
-      constructor
-    next =>
-      apply BigStep.whileFalse
-      rw [← AsBool.optimize_ok]
-      assumption
+    split <;> try simp
+    apply BigStep.whileFalse
+    rw [← Expr.optimize_ok]
+    assumption
   | whileTrue isTrue bodyStep nextStep ih1 ih2 =>
     split
     next c isZero =>
-      rw [AsBool.optimize_ok, isZero] at isTrue
-      cases isTrue.not_const_0_true
+      rw [Expr.optimize_ok, isZero] at isTrue
+      simp at isTrue
     next c isNotZero =>
       apply BigStep.whileTrue
-      . rw [← AsBool.optimize_ok]
+      . rw [← Expr.optimize_ok]
         assumption
       . apply ih1
       . simp [optimize] at ih2
         assumption
 
-
-
-
 inductive SmallStep : Env → Stmt → Env → Stmt → Prop where
   | seq1 : SmallStep ρ s1 ρ' s1' → SmallStep ρ (.seq s1 s2) ρ' (.seq s1' s2)
   | seq2 : SmallStep ρ (.seq .skip s2) ρ s2
   | assign : e.eval ρ = some v → SmallStep ρ (.assign x e) (ρ.set x v) .skip
-  | ifTrue : AsBool ρ c true → SmallStep ρ (.if c s1 s2) ρ s1
-  | ifFalse : AsBool ρ c false → SmallStep ρ (.if c s1 s2) ρ s2
-  | whileTrue : AsBool ρ c true → SmallStep ρ (.while c s) ρ (.seq s (.while c s))
-  | whileFalse : AsBool ρ c false → SmallStep ρ (.while c s) ρ .skip
+  | ifTrue : Truthy (c.eval ρ) → SmallStep ρ (.if c s1 s2) ρ s1
+  | ifFalse : Falsy (c.eval ρ) → SmallStep ρ (.if c s1 s2) ρ s2
+  | whileTrue : Truthy (c.eval ρ) → SmallStep ρ (.while c s) ρ (.seq s (.while c s))
+  | whileFalse : Falsy (c.eval ρ) → SmallStep ρ (.while c s) ρ .skip
 
-open Stmt.Syntax in
 inductive SmallStep' : Env → Stmt → Env → Stmt → Prop where
   | seq1 :
     SmallStep' ρ s1 ρ' s1' →
     SmallStep'
-      ρ  (program {~s1 ; ~s2})
-      ρ' (program {~s1'; ~s2})
+      ρ  (program {~s1 ~s2})
+      ρ' (program {~s1 ~s2})
   | seq2 :
     SmallStep'
       ρ (program {skip; ~s2})
       ρ s2
-  | assign :
+  | assign : {e : Expr} →
     e.eval ρ = some v →
     SmallStep'
-      ρ           program {~x := ~e}
-      (ρ.set x v) program {skip}
+      ρ           (program {~x := ~e;})
+      (ρ.set x v) (program {skip;})
   | ifTrue :
-    AsBool ρ c true →
+    Truthy (c.eval ρ) →
     SmallStep'
-      ρ program {if (~c) {~s1} else {~s2}}
+      ρ (program {if (~c) {~s1} else {~s2}})
       ρ s1
   | ifFalse :
-    AsBool ρ c false →
+    Falsy (c.eval ρ) →
     SmallStep'
-      ρ program {if (~c) {~s1} else {~s2}}
+      ρ (program {if (~c) {~s1} else {~s2}})
       ρ s2
   | whileTrue :
-    AsBool ρ c true →
+    Truthy (c.eval ρ) →
     SmallStep'
-      ρ program {while (~c) {~s}}
-      ρ program {~s; while(~c) {~s}}
+      ρ (program {while (~c) {~s}})
+      ρ (program {~s while(~c) {~s}})
   | whileFalse :
-    AsBool ρ c false →
+    Falsy (c.eval ρ) →
     SmallStep'
-      ρ program {while (~c) {~s}}
-      ρ .skip
+      ρ (program {while (~c) {~s}})
+      ρ (program {skip;})
 
 structure ValidStep (ρ : Env) (s : Stmt) where
   env : Env
@@ -627,7 +261,7 @@ instance : Repr (ValidStep ρ s) where
 inductive SmallSeq : Nat → Env → Stmt → Env → Stmt → Type where
   | done : SmallSeq n ρ .skip ρ .skip
   | noGas : SmallSeq 0 ρ s ρ s
-  | crash : ¬IsSkip s → (¬ ∃ ρ' s', SmallStep ρ s ρ' s') → SmallSeq n ρ s ρ s
+  | crash : s ≠ .skip → (¬ ∃ ρ' s', SmallStep ρ s ρ' s') → SmallSeq n ρ s ρ s
   | step : SmallStep ρ s ρ' s' → SmallSeq n ρ' s' ρ'' s'' → SmallSeq (n + 1) ρ s ρ'' s''
 
 def SmallSeq.render (vars : List String) : SmallSeq n ρ s ρ' s' → Std.Format
@@ -642,11 +276,10 @@ def SmallSeq.final (vars : List String) (_ : SmallSeq n ρ s ρ' s') : Std.Forma
 
 def smallStep (ρ : Env) (s : Stmt) : ValidStep ρ s ⊕ (Inhabited <| ValidStep ρ s → False) :=
   match s with
-  | .skip => .inr ⟨nofun⟩
-  | .seq s1 s2 =>
-    if h : IsSkip s1 then
-      let .isSkip := h
-      .inl ⟨_, _, .seq2⟩
+  | program{skip;} => .inr ⟨nofun⟩
+  | program{ ~s1 ~s2} =>
+    if h : s1 = .skip then
+      .inl ⟨_, _, h ▸ SmallStep.seq2⟩
     else
       match smallStep ρ s1 with
       | .inl ⟨_, _, step⟩ => .inl ⟨_, _, .seq1 step⟩
@@ -668,9 +301,9 @@ def smallStep (ρ : Env) (s : Stmt) : ValidStep ρ s ⊕ (Inhabited <| ValidStep
       cases step
       next prf => rw [h] at prf; contradiction
   | .while c s =>
-    if h : AsBool ρ c true then
+    if h : Truthy (c.eval ρ) then
       .inl <| ⟨_, _, .whileTrue h⟩
-    else if h' : AsBool ρ c false then
+    else if h' : Falsy (c.eval ρ) then
       .inl <| ⟨_, _, .whileFalse h'⟩
     else
       .inr <| by
@@ -678,9 +311,9 @@ def smallStep (ρ : Env) (s : Stmt) : ValidStep ρ s ⊕ (Inhabited <| ValidStep
         intro ⟨_, _, step⟩
         cases step <;> contradiction
   | .if c s1 s2 =>
-    if h : AsBool ρ c true then
+    if h : Truthy (c.eval ρ) then
       .inl ⟨_, _, .ifTrue h⟩
-    else if h' : AsBool ρ c false then
+    else if h' : Falsy (c.eval ρ) then
       .inl ⟨_, _, .ifFalse h'⟩
     else
       .inr <| by
@@ -690,7 +323,7 @@ def smallStep (ρ : Env) (s : Stmt) : ValidStep ρ s ⊕ (Inhabited <| ValidStep
 
 
 def runFor (n : Nat) (ρ : Env) (s : Stmt) : (ρ' : Env) × (s' : Stmt) × SmallSeq n ρ s ρ' s' :=
-  if h : IsSkip s then
+  if h : s = .skip then
     ⟨ρ, s, by cases h; apply SmallSeq.done⟩
   else
     match n with
@@ -704,27 +337,31 @@ def runFor (n : Nat) (ρ : Env) (s : Stmt) : (ρ' : Env) × (s' : Stmt) × Small
         apply contra
         constructor; assumption
 
-open Stmt.Syntax in
 def fib : Stmt := program {
   x := 0; y := 0;
   while (n > 0) {
     x := y;
     y := y + n;
-    n := n + - 1
+    n := n + - 1;
   }
 }
 
 #eval let ρ' := runFor 20 (Env.init 42 |>.set "n" 6 |>.set "x" 0) fib |>.fst; (ρ' "x", ρ' "y", ρ' "n")
 
-open Stmt.Syntax in
-#eval smallStep (Env.init 99 |>.set "n" 0) program{ while (n > 0) {n := n - 1} } |> (match · with | .inl x => some x | .inr _ => none)
+#eval smallStep (Env.init 99 |>.set "n" 0) (program{ while (n > 0) {n := n - 1;} }) |> (match · with | .inl x => some x | .inr _ => none)
 
 #eval
   let ρ' := runFor 200 (Env.init 42 |>.set "n" 6 |>.set "x" 0) fib
   ρ'.snd.snd.final ["x", "y", "n"]
 
+@[simp] theorem BitVec.shiftRight_shiftRight' (w : Nat) (x : BitVec w) (n m : BitVec w)
+    (h : (n + m).toNat = n.toNat + m.toNat) :
+    (x >>> n) >>> m = x >>> (n + m) := by
+  show (x >>> n.toNat) >>> m.toNat = x >>> (n + m).toNat
+  simp [h, BitVec.shiftRight_shiftRight]
+
 def runFor' (n : Nat) (ρ : Env) (s : Stmt) : Option Env :=
-  if IsSkip s then
+  if let program {skip;} := s then
     some ρ
   else
     match n with
@@ -735,26 +372,35 @@ def runFor' (n : Nat) (ρ : Env) (s : Stmt) : Option Env :=
         runFor' n' ρ' s'
       | .inr _ => none
 
-open Stmt.Syntax in
 def popcount : Stmt := program {
   x := x - ((x >>> 1) &&& 0x55555555);
   x := (x &&& 0x33333333) + ((x >>> 2) &&& 0x33333333);
   x := (x + (x >>> 4)) &&& 0x0F0F0F0F;
   x := x + (x >>> 8);
   x := x + (x >>> 16);
-  x := x &&& 0x0000003F
+  x := x &&& 0x0000003F;
 }
 
-open Stmt.Syntax in
 def popcountLoop : Stmt := program {
   i := 32;
   count := 0;
   while (i > 0) {
     count := count + (x &&& 1);
     i := i - 1;
-    x := x >>> 1
-  };
-  x := count
+    x := x >>> 1;
+  }
+  x := count;
+}
+
+def popcountLoop2 : Stmt := program {
+  i := 32;
+  count := 0;
+  while (i > 0) {
+    count := count + (x &&& 80000000);
+    i := i - 1;
+    x := x <<< 1;
+  }
+  x := count;
 }
 
 def pop_spec' (x : BitVec 32) : BitVec 32 :=
@@ -778,22 +424,133 @@ where
 #eval (runFor' 11 (Env.init 1230123) popcountLoop) |>.map (· "x")
 
 
-set_option maxRecDepth 2000 in
+theorem Env.set_order {ρ : Env} : x ≠ y → (ρ.set x v1 |>.set y v2) = (ρ.set y v2 |>.set x v1) := by
+  intro h
+  funext z
+  simp [Env.set]
+  split <;> split
+  . subst_eqs; contradiction
+  . rfl
+  . rfl
+  . rfl
+
+theorem Char.lt_irrefl (c : Char) : ¬ (c < c) := by
+  simp [LT.lt]
+  intro lt
+  unfold Char.lt at lt
+  unfold instLTUInt32 at lt
+  simp_all
+  unfold instLTFin at lt
+  simp_all
+
+
+theorem Env.set_reorder {ρ : Env} : x < y → (ρ.set y v2 |>.set x v1) = (ρ.set x v1 |>.set y v2) := by
+  intro h
+  have : x ≠ y := by
+    simp [LT.lt, List.lt] at h
+    intro eq
+    rw [eq] at h
+    apply List.lt_irrefl' Char.lt_irrefl y.data h
+  funext z
+  simp [Env.set]
+  split <;> split
+  . subst_eqs; contradiction
+  . rfl
+  . rfl
+  . rfl
+
+@[simp]
+theorem Env.get_init : (Env.init v).get x = v := by rfl
+
+@[simp]
+theorem Env.get_set_same {ρ : Env} : (ρ.set x v).get x = v := by
+  simp [get, set]
+
+@[simp]
+theorem Env.get_set_different {ρ : Env} : x ≠ y → (ρ.set x v).get y = ρ.get y := by
+  intros
+  simp [get, set, *]
+
+
+-- These seem like they should be simprocs :-)
+
+@[simp]
+theorem Env.set_dedup {ρ : Env} :  (ρ.set x v1 |>.set x v2) = (ρ.set x v2) := by
+  funext z
+  simp [Env.set]
+  split <;> simp
+
+@[simp]
+theorem Env.set_dedup2 {ρ : Env} : (ρ.set x v1 |>.set y v |>.set x v2) = (ρ.set y v |>.set x v2) := by
+  funext z
+  simp [Env.set]
+  split <;> simp
+
+@[simp]
+theorem Env.set_dedup3 {ρ : Env} : (ρ.set x v1 |>.set y v |>.set z v' |>.set x v2) = (ρ.set y v |>.set z v' |>.set x v2) := by
+  funext z
+  simp [Env.set]
+  repeat split <;> try rfl
+
+@[simp]
+theorem Expr.eval_const : Expr.eval ρ (.const v) = some v := by simp [Expr.eval]
+
 theorem popCount_correct : ∃ ρ, (runFor' 11 (Env.init x) popcount) = some ρ ∧ ρ "x" = pop_spec' x := by
-  simp (config:={decide := true}) [runFor', popcount, smallStep, Env.init, Expr.eval, BinOp.apply, Env.set, OfNat.ofNat]
-  dsimp [pop_spec', pop_spec'.go]
-  unfold Value at x
-  unfold Value
+  simp [runFor', popcount, smallStep, Env.init, Expr.eval, Expr.BinOp.apply, Env.set, pop_spec', pop_spec'.go, Value]
   bv_decide
 
-/- This doesn't work (so much defeq!)
-set_option trace.bv true
-set_option maxRecDepth 2000 in
-set_option maxHeartbeats 2000000 in
-theorem popCountLoop_correct : ∃ ρ, (runFor' 240 (Env.init x) popcountLoop) = some ρ ∧ ρ "x" = pop_spec' x := by
-  simp (config:={decide := true}) [runFor', popcount, smallStep, Env.init, Expr.eval, BinOp.apply, Env.set, OfNat.ofNat, AsBool]
-  dsimp [pop_spec', pop_spec'.go]
-  unfold Value at x
-  unfold Value
+#eval 5
+
+@[simp]
+theorem BitVec.and_self {x : BitVec 32} : x &&& x = x := by
   bv_decide
--/
+
+@[simp]
+theorem BitVec.and_self_ofNat {x : Nat} : BitVec.ofNat 32 x &&& BitVec.ofNat 32 x = BitVec.ofNat 32 x := by
+  simp
+
+macro "cleanup_env" : tactic =>
+  `(tactic| (
+    (repeat conv in Env.get "x" (Env.set "i" _ _) => rw [Env.get_set_different (by decide)]);
+    (repeat conv in Env.get "x" (Env.set "count" _ _) => rw [Env.get_set_different (by decide)]);
+    (repeat conv in Env.get "i" (Env.set "x" _ _) => rw [Env.get_set_different (by decide)]);
+    (repeat conv in Env.get "i" (Env.set "count" _ _) => rw [Env.get_set_different (by decide)]);
+    (repeat conv in Env.get "count" (Env.set "x" _ _) => rw [Env.get_set_different (by decide)]);
+    (repeat conv in Env.get "count" (Env.set "i" _ _) => rw [Env.get_set_different (by decide)]);
+    (repeat rw [Env.get_set_same]))
+  )
+
+
+-- This is an horrible hack that gets it to compute. Why aren't the simp lemmas firing?
+set_option maxHeartbeats 2000000 in
+set_option maxRecDepth 1024 in
+set_option trace.bv true in
+theorem popCountLoop_correct : ∃ ρ, (runFor' 240 (Env.init x) popcountLoop) = some ρ ∧ ρ.get "x" = pop_spec' x := by
+  have : "count" ≠ "i" := by decide
+  have : "count" ≠ "x" := by decide
+  have : "x" ≠ "i" := by decide
+  have : 1#32 ≠ 0#32 := by decide
+  unfold popcountLoop
+  -- Not sure why I need to call repeat multiple times...
+  repeat (unfold runFor'; simp [smallStep, Expr.eval, Expr.BinOp.apply, *]; cleanup_env)
+  repeat (unfold runFor'; simp [smallStep, Expr.eval, Expr.BinOp.apply, *]; cleanup_env)
+  repeat (unfold runFor'; simp [smallStep, Expr.eval, Expr.BinOp.apply, *]; cleanup_env)
+  simp [pop_spec', pop_spec'.go, Value]
+  -- Holds by reflexivity; both implement the same algorithm
+
+set_option maxHeartbeats 2000000 in
+set_option maxRecDepth 1024 in
+set_option trace.bv true in
+theorem popCountLoop2_correct : ∃ ρ, (runFor' 240 (Env.init x) popcountLoop2) = some ρ ∧ ρ.get "x" = pop_spec' x := by
+  have : "count" ≠ "i" := by decide
+  have : "count" ≠ "x" := by decide
+  have : "x" ≠ "i" := by decide
+  have : 1#32 ≠ 0#32 := by decide
+  unfold popcountLoop2
+  -- Not sure why I need to call repeat multiple times...
+  repeat (unfold runFor'; simp [smallStep, Expr.eval, Expr.BinOp.apply, *]; cleanup_env)
+  repeat (unfold runFor'; simp [smallStep, Expr.eval, Expr.BinOp.apply, *]; cleanup_env)
+  repeat (unfold runFor'; simp [smallStep, Expr.eval, Expr.BinOp.apply, *]; cleanup_env)
+  simp [pop_spec', pop_spec'.go, Value]
+  -- Why doesn't this work? Is there a bug?
+  bv_decide
