Imp/Expr.lean
@@ -1,0 +1,132 @@
+import Lean.PrettyPrinter.Delaborator
+
+open Lean
+open Lean.PrettyPrinter Parenthesizer
+
+
+namespace Imp.Expr
+
+declare_syntax_cat varname
+syntax ident : varname
+syntax:max "~" term:max : varname
+
+syntax "var " "{" varname "}" : term
+
+macro_rules
+  | `(var { $x:ident }) => `(term|$(quote x.getId.toString))
+  | `(var { ~$stx }) => pure stx
+
+inductive UnOp where
+  | neg
+  | not
+deriving Repr, DecidableEq
+
+inductive BinOp where
+  | plus | minus | times | div
+  | lsh | rsh
+  | band | bor
+  | and | or
+  | lt | le | eq
+deriving Repr, DecidableEq
+
+end Expr
+
+inductive Expr where
+  | const (i : BitVec 32)
+  | var (name : String)
+  | un (op : Expr.UnOp) (e : Expr)
+  | bin (op : Expr.BinOp) (e1 e2 : Expr)
+deriving Repr, DecidableEq
+
+namespace Expr.Syntax
+
+declare_syntax_cat exp
+syntax varname : exp
+/-- Numeric constant -/
+syntax num : exp
+/-- Arithmetic complement -/
+syntax:75 "-" exp:75 : exp
+/-- Addition -/
+syntax:65 exp:65 " + " exp:66 : exp
+/-- Multiplication -/
+syntax:70 exp:70 " * " exp:71 : exp
+/-- Subtraction -/
+syntax:65 exp:65 " - " exp:66 : exp
+/-- Division -/
+syntax:65 exp:65 " / " exp:66 : exp
+
+-- todo precs
+syntax:55 exp:55 " <<< " exp:56 :exp
+syntax:55 exp:55 " >>> " exp:56 :exp
+syntax:55 exp:55 " &&& " exp:56 :exp
+syntax:55 exp:55 " ||| " exp:56 :exp
+
+--todo precs for these
+/-- Boolean conjunction -/
+syntax:65 exp:65 " && " exp:66 : exp
+/-- Boolean disjunction -/
+syntax:65 exp:65 " || " exp:66 : exp
+
+/-- Boolean negation -/
+syntax:75 "!" exp:75 : exp
+/-- Less than -/
+syntax:50 exp:50 " < " exp:50 : exp
+/-- Less than or equal to -/
+syntax:50 exp:50 " ≤ " exp:50 : exp
+/-- Equal -/
+syntax:50 exp:50 " = " exp:50 : exp
+/-- Equal -/
+syntax:50 exp:50 " == " exp:50 : exp
+/-- Greater than or equal to -/
+syntax:50 exp:50 " ≥ " exp:50 : exp
+/-- Greater than -/
+syntax:50 exp:50 " > " exp:50 : exp
+
+/-- Parens -/
+syntax "(" exp ")" : exp
+
+syntax:max "~" term:max : exp
+
+syntax "lean " "{ " term " }" : exp
+
+syntax "expr " "{ " exp " }" : term
+
+open Lean in
+macro_rules
+  | `(expr{$x:ident}) => `(Expr.var $(quote x.getId.toString))
+  | `(expr{$n:num}) => `(Expr.const $(quote n.getNat))
+
+  | `(expr{-$e}) => `(Expr.un .neg expr{$e})
+  | `(expr{!$e}) => `(Expr.un .not expr{$e})
+
+  | `(expr{$e1 + $e2}) => `(Expr.bin .plus expr{$e1} expr{$e2})
+  | `(expr{$e1 * $e2}) => `(Expr.bin .times expr{$e1} expr{$e2})
+  | `(expr{$e1 - $e2}) => `(Expr.bin .minus expr{$e1} expr{$e2})
+  | `(expr{$e1 / $e2}) => `(Expr.bin .div expr{$e1} expr{$e2})
+
+  | `(expr{$e1 >>> $e2}) => `(Expr.bin .rsh expr{$e1} expr{$e2})
+  | `(expr{$e1 <<< $e2}) => `(Expr.bin .lsh expr{$e1} expr{$e2})
+  | `(expr{$e1 ||| $e2}) => `(Expr.bin .bor expr{$e1} expr{$e2})
+  | `(expr{$e1 &&& $e2}) => `(Expr.bin .band expr{$e1} expr{$e2})
+
+
+  | `(expr{$e1 && $e2}) => `(Expr.bin .and expr{$e1} expr{$e2})
+  | `(expr{$e1 || $e2}) => `(Expr.bin .or expr{$e1} expr{$e2})
+
+  | `(expr{$e1 < $e2}) => `(Expr.bin .lt expr{$e1} expr{$e2})
+  | `(expr{$e1 ≤ $e2}) => `(Expr.bin .le expr{$e1} expr{$e2})
+  | `(expr{$e1 == $e2}) => `(Expr.bin .eq expr{$e1} expr{$e2})
+  | `(expr{$e1 ≥ $e2}) => `(Expr.bin .le expr{$e2} expr{$e1})
+  | `(expr{$e1 > $e2}) => `(Expr.bin .lt expr{$e2} expr{$e1})
+  | `(expr{($e)}) => `(expr{$e})
+  | `(expr{~$stx}) => pure stx
+
+-- Shamelessly stolen from Lean's term parenthesizer
+@[category_parenthesizer exp]
+def exp.parenthesizer : CategoryParenthesizer | prec => do
+  maybeParenthesize `exp true wrapParens prec $
+    parenthesizeCategoryCore `exp prec
+where
+  wrapParens (stx : Syntax) : Syntax := Unhygienic.run do
+    let pstx ← `(($(⟨stx⟩)))
+    return pstx.raw.setInfo (SourceInfo.fromRef stx)
