Imp/Expr/Eval.lean
@@ -1,0 +1,57 @@
+import Imp.Expr
+
+namespace Imp
+
+abbrev Value := BitVec 32
+
+def Env := String → Value
+
+namespace Env
+
+def set (x : String) (v : Value) (ρ : Env) : Env :=
+  fun y => if x == y then v else ρ y
+
+def get (x : String) (ρ : Env) : Value :=
+  ρ x
+
+def init (i : Value) : Env := fun _ => i
+
+end Env
+
+namespace Expr
+
+def freeVars : Expr → List String
+  | .const _ => []
+  | .var x => [x]
+  | .un _ e => e.freeVars
+  | .bin _ e1 e2 => e1.freeVars ++ e2.freeVars
+
+def UnOp.apply : UnOp → Value → Option Value
+  | .neg, x => some (- x)
+  | .not, x => some (if x == 0 then 1 else 0)
+
+def BinOp.apply : BinOp → Value → Value → Option Value
+  | .plus, x, y => some (x + y)
+  | .minus, x, y => some (x - y)
+  | .times, x, y => some (x * y)
+  | .lsh, x, y => some (x <<< y)
+  | .rsh, x, y => some (x >>> y)
+  | .band, x, y => some (x &&& y)
+  | .bor, x, y => some (x ||| y)
+  | .div, x, y => if y == 0 then none else some (x / y)
+  | .and, x, y => some (if x == 0 then 0 else y)
+  | .or, x, y => some (if x == 0 then y else x)
+  | .eq, x, y => some (if x == y then 1 else 0)
+  | .le, x, y => some (if x ≤ y then 1 else 0)
+  | .lt, x, y => some (if x < y then 1 else 0)
+
+def eval (ρ : Env) : Expr → Option Value
+  | .const i => some i
+  | .var x => ρ.get x
+  | .un op e => do
+    let v ← e.eval ρ
+    op.apply v
+  | .bin op e1 e2 => do
+    let v1 ← e1.eval ρ
+    let v2 ← e2.eval ρ
+    op.apply v1 v2
