Imp/Stmt.lean
@@ -1,0 +1,34 @@
+import Imp.Expr
+
+namespace Imp
+
+inductive Stmt where
+  | skip
+  | seq (stmt1 stmt2 : Stmt)
+  | assign (name : String) (val : Expr)
+  | if (cond : Expr) (ifTrue ifFalse : Stmt)
+  | while (cond : Expr) (body : Stmt)
+deriving Repr, DecidableEq
+
+namespace Stmt
+
+declare_syntax_cat stmt
+scoped syntax "skip" ";" : stmt
+scoped syntax stmt ppDedent(ppLine stmt) : stmt
+scoped syntax varname " := " exp ";" : stmt
+scoped syntax "if " "(" exp ")" ppHardSpace "{" ppLine stmt ppDedent(ppLine "}" ppHardSpace "else" ppHardSpace "{") ppLine stmt ppDedent(ppLine "}") : stmt
+scoped syntax "while " "(" exp ")" ppHardSpace "{" ppLine stmt ppDedent(ppLine "}") : stmt
+scoped syntax:max "~" term:max : stmt
+
+syntax "program" ppHardSpace "{" ppLine stmt ppDedent(ppLine "}") : term
+
+
+open Lean in
+macro_rules
+  | `(program { skip; }) => `(Stmt.skip)
+  | `(program { $s1 $s2 }) => `(Stmt.seq (program {$s1}) (program {$s2}))
+  | `(program { $x:varname := $e;}) =>
+      `(Stmt.assign var {$x} expr {$e})
+  | `(program { if ($c) {$s1} else {$s2} }) => `(Stmt.if expr{$c} (program{$s1}) (program{$s2}))
+  | `(program { while ($c) {$s} }) => `(Stmt.while expr{$c} (program{$s}))
+  | `(program { ~$stx }) => pure stx
