Imp/Stmt/Delab.lean
@@ -1,0 +1,137 @@
+import Lean.PrettyPrinter.Delaborator
+import Imp.Stmt
+import Imp.Expr
+import Imp.Expr.Delab
+
+open Lean PrettyPrinter.Delaborator SubExpr
+
+namespace Imp.Stmt.Delab
+
+open Imp.Stmt
+open Imp.Expr.Delab
+
+partial def delabStmtInner : DelabM (TSyntax `stmt) := do
+  let e ← getExpr
+  let stx ←
+    match_expr e with
+    | Stmt.skip => `(stmt| skip;)
+    | Stmt.seq _ _ =>
+      let s1 ← withAppFn <| withAppArg delabStmtInner
+      let s2 ← withAppArg delabStmtInner
+      `(stmt| $s1 $s2)
+    | Stmt.assign _ _ =>
+      let x ← withAppFn <| withAppArg delabNameInner
+      let e ← withAppArg delabExprInner
+      `(stmt| $x:varname := $e;)
+    | Stmt.while _ _ =>
+      let c ← withAppFn <| withAppArg delabExprInner
+      let body ← withAppArg delabStmtInner
+      `(stmt| while ($c) { $body })
+    | Stmt.if _ _ _ =>
+      let c ← withAppFn <| withAppFn <| withAppArg delabExprInner
+      let t ← withAppFn <| withAppArg delabStmtInner
+      let f ← withAppArg delabStmtInner
+      `(stmt| if ($c) { $t } else { $f })
+    | _ =>
+      `(stmt| ~$(← delab))
+  annAsTerm stx
+
+@[delab app.Imp.Stmt.skip, delab app.Imp.Stmt.seq, delab app.Imp.Stmt.while, delab app.Imp.Stmt.assign, delab App.Imp.Stmt.if]
+partial def delabStmt : Delab := do
+  -- This delaborator only understands a certain arity - bail if it's incorrect
+  guard <| match_expr ← getExpr with
+    | Stmt.skip => true
+    | Stmt.seq _ _ => true
+    | Stmt.while _ _ => true
+    | Stmt.assign _ _ => true
+    | Stmt.if _ _ _ => true
+    | _ => false
+  match ← delabStmtInner with
+  | `(stmt|~$e) => pure e
+  | s => `(term|program{$s})
+
+/-- info: Imp.Stmt.skip : Stmt -/
+#guard_msgs in
+#check Stmt.skip
+
+/--
+info: program {
+  skip;
+} : Stmt
+-/
+#guard_msgs in
+#check program {skip;}
+
+/--
+info: program {
+  skip;
+  skip;
+} : Stmt
+-/
+#guard_msgs in
+#check program {skip; skip;}
+
+/--
+info: program {
+  skip;
+  skip;
+  x := 5;
+} : Stmt
+-/
+#guard_msgs in
+#check program {skip; skip; x := 5;}
+
+/--
+info: program {
+  skip;
+  if (0 < x) {
+    x := x - 1;
+  } else {
+    skip;
+  }
+} : Stmt
+-/
+#guard_msgs in
+#check program {skip; if (x > 0) { x := x - 1;} else {skip;}}
+
+/--
+info: program {
+  skip;
+  while (0 < x) {
+      x := x - 1;
+    }
+  if (x) {
+    skip;
+  } else {
+    while (5 < x) {
+      skip;
+      skip;
+    }
+  }
+} : Stmt
+-/
+#guard_msgs in
+#check program {skip; while (x > 0) { x := x - 1;} if (x) {skip;} else {while (x > 5) {skip; skip;}}}
+
+/--
+info: let s :=
+  program {
+    skip;
+  };
+program {
+  skip;
+  while (0 < x) {
+      x := x - 1;
+    }
+  if (x) {
+    skip;
+  } else {
+    while (5 < x) {
+      skip;
+      ~s
+    }
+  }
+} : Stmt
+-/
+#guard_msgs in
+#check let s := program {skip;}; program {skip; while (x > 0) { x := x - 1;} if (x) {skip;} else {while (x > 5) {skip; ~s}}}
